examples/sgx/Interpreter.fst
@@ -2,20 +2,15 @@
 module Interpreter
 
 open FStar.Buffer
-open FStar.ST
+open FStar.HST
 open FStar.UInt64
-open FStar.List
+open FStar.List.Tot
 open Util
 open Ast
 open Test
 open SGXState
 
 exception Halt
-
-let dword = UInt64.t
-let word = UInt32.t
-let address = UInt64.t
-let offset = UInt64.t
 
 (*
 val STX.Halt: unit -> STX 'a 
@@ -27,30 +22,39 @@ assume val search: (buffer dword)->(addr:address)-> bool
 
 type memaccess =
  |MkMemAccess: 
-	      read: (cpuregstate -> string) -> (* Helper function to read registers, used by store *)
-  	      load: (word -> address -> dword) ->
-  	      store:(word -> address-> dword -> cpuregstate ->unit)->
-	      decode:(program ->address->(list stmt))->memaccess
+	      read: (string->cpuregstate -> dword) -> (* Helper function to read registers, used by store *)
+  	      (* load: (word -> address -> STL dword  ) -> *)
+  	      load: (word -> address -> STL dword (requires (fun h -> true)) (ensures (fun h0 r h1 -> true))) -> 
+  	      store:(word -> address-> dword -> cpuregstate ->STL unit (requires (fun h -> true)) (ensures (fun h0 r h1 -> true))) ->
+	      decode:(program ->address->Tot (list stmt))->memaccess
 
-val defensive: (buffer dword)->(list dword) ->address-> address->address->address->address->memaccess
+val defensive: (buffer dword)->(buffer dword) ->address-> address->address->address->address->STL memaccess
+									(requires (fun h -> true)) 
+									(ensures (fun h0 r h1 -> true)) 
 let defensive buf calltable base wbmapstart ucodestart uheapstart ustackstart = 
   let read' (regname:string) (env:cpuregstate) =
+	(*
  	let rec search_reg regname = function
-		  |[] -> raise Halt
+		  |[] -> (* raise Halt *) 0uL
 		  |(MkReg regname' value)::tail -> if regname' = regname then
 								value
 							else
 								search_reg regname tail
 	in
 	search_reg regname (get_reg_list env)
+	*)
+	0uL
   in
-  let load' (n:word) (addr:address) = 
-       let idx = (sub addr base) in
+  let load'(n:word) (addr:address): STL dword
+	(requires (fun h -> true))
+	(ensures (fun h0 r h1 -> true))
+	  =
+       (let idx = (sub addr base) in
        let wordidx = (cast_to_word idx) in
-       (* Buffer.index buf wordidx *)
-	()
+       Buffer.index buf wordidx 
+       )
     in
-  let store' (n:word) (v:dword) (addr:address) (env:cpuregstate) =
+  let store' (n:word) (addr:address) (v:dword) (env:cpuregstate) =
      if (gt addr  wbmapstart) && (lt addr  ucodestart) then
 	(* addr is in write-bitmap, get the index
 	   i.e. bitmapindex represents the address whose permission
@@ -63,23 +67,24 @@ let defensive buf calltable base wbmapstart ucodestart uheapstart ustackstart =
 	  2. Check that 'bitmapindex' is less than [|rbp |] 
 	*)
 	let currentframestart = (read' "rbp" env) in
-	if (lt bitmapindex currentframestart) then	
+
+	if (lt bitmapindex currentframestart) then
 	       let idx = (sub addr base) in
 	       let wordidx = (cast_to_word idx) in
-        	(* Buffer.upd buf wordidx v*)
-		()
+        	Buffer.upd buf wordidx v
 	else
-		raise Halt
+		(* raise Halt *)
+		()
     else if (gt addr uheapstart) && (lt addr  ustackstart) then
 	(* Address is in UHeap... Check that bitmap is set *)  
 	let isbitmapset = get_bitmap_set base wbmapstart addr in
 	if isbitmapset then
 	       let idx = (sub addr base) in
 	       let wordidx = (cast_to_word idx) in
-        	(* Buffer.upd buf wordidx v*)
-		()
+        	Buffer.upd buf wordidx v
 	else
-		raise Halt
+		(* raise Halt *)
+		()
  
     else if (gt addr ustackstart) && (lt addr (read' "rbp" env))  then
 	(* Address belongs to older stack frames *)  
@@ -87,50 +92,50 @@ let defensive buf calltable base wbmapstart ucodestart uheapstart ustackstart =
 	if isbitmapset then
 	       let idx = (sub addr base) in
 	       let wordidx = (cast_to_word idx) in
-        	(* Buffer.upd buf wordidx v*)
-		()
+         	Buffer.upd buf wordidx v
 	else
-		raise Halt
+		(* raise Halt *)
+		()
 
     else if (gt addr (read' "rbp" env)) && (lt addr (read' "rsp" env))  then
 	(* Address belongs to current stack frames *)  
 	       let idx = (sub addr base) in
 	       let wordidx = (cast_to_word idx) in
-        	(* Buffer.upd buf wordidx v*)
-		()
+                Buffer.upd buf wordidx v
     in
   let decode' myprogram instraddr = 
-	let iscallable = search calltable instraddr in
+	let iscallable = search_func calltable instraddr in
 	if  iscallable then
 		let func_name = get_func_name calltable instraddr in
 		(* Fetches instructions from start to end *)
 		let stlist = get_stmt_list func_name myprogram in
 			stlist
 	else
-		raise Halt
+		(* raise Halt *)
+			[]
     in	
 
    MkMemAccess read' load' store' decode'
 	
 let get_register_name = function
  | Register r -> r
- | _ -> raise Halt
+ | _ -> (* raise Halt *) ""
 
-val update: string -> dword->cpuregstate->cpuregstate
+val update: string -> dword->cpuregstate->Tot cpuregstate
 let update (regname:string) (value:dword) (env:cpuregstate) =
- let rec loop pre = function
-	| [] -> raise Halt
-	| MkReg(regname', v)::tail -> if regname' = regname then
-						(pre @ [MkReg (regname, value)] @ tail)
+ let rec loop (pre:list register) (post:list register) :(Tot cpuregstate) = match post with
+	| [] -> (* raise Halt *) (Mkcpuregstate [])
+	| (MkReg regname' v)::tail -> if regname' = regname then
+						(Mkcpuregstate (pre@[MkReg regname value] @ tail))
 					  else
-						loop (pre@[(MkReg (regname,v))]) tail 
-	in loop [] env
+						loop (pre@[(MkReg regname v)]) tail 
+	in loop [] (get_reg_list env)
 						
 
-val eval: cpuregstate -> exp -> dword
+val eval: cpuregstate -> exp -> Tot dword
 let eval (env:cpuregstate) = function
- | Register r ->  let rec search_reg regname = function
-		  |[] -> raise Halt
+ | Register r ->  let rec search_reg (regname:string) (li:list register) :Tot dword = match li with
+		  |[] -> (* raise Halt *) 0uL
 		  |(MkReg regname' value)::tail -> if regname' = regname then
 								value
 							else
@@ -139,8 +144,17 @@ let eval (env:cpuregstate) = function
  | Constant n -> n
 
 
-val step : cpuregstate  -> program -> stmt -> ST cpuregstate
-val steps : cpuregstate -> program -> (list stmt) -> ST cpuregstate
+val step : cpuregstate  ->memaccess-> program -> stmt -> STL cpuregstate 
+			(requires (fun h -> true))
+			(ensures (fun h0 r h1 -> true))
+val steps : cpuregstate ->memaccess-> program -> (list stmt) -> STL cpuregstate
+			(requires (fun h -> true))
+			(ensures (fun h0 r h1 -> true))
+assume val fold_right: ('a -> 'b -> STL 'b
+			(requires (fun h -> true))
+			(ensures (fun h0 r h1 -> true))) -> list 'a -> 'b -> STL 'b
+								(requires (fun h -> true))
+								(ensures (fun h0 r h1 -> true))
 let rec step (env:cpuregstate) (defensivememop:memaccess) (myprogram:program) = function 
   | Skip -> env
   | Store(n, ea, ev)-> 
@@ -150,9 +164,10 @@ let rec step (env:cpuregstate) (defensivememop:memaccess) (myprogram:program) = 
        env
   | Load (reg, n, ea) ->
        let a = eval env ea in
-       let value = defensivememop.load (cast_to_word n) a in
+       let wordn = (cast_to_word n) in
+       let value = defensivememop.load wordn a in
        let regname = get_register_name reg in
-       let env' = update regname value in
+       let env' = update regname value env in
        env'
   | Call e ->
        let fentry = eval env e in
@@ -163,37 +178,40 @@ let rec step (env:cpuregstate) (defensivememop:memaccess) (myprogram:program) = 
 	steps env defensivememop myprogram stmtlist 
   | If (e, truli, falsli) ->
 	let boolval = eval env e in
-	if boolval then
+	if not (eq boolval 0uL)  then
 		steps env defensivememop myprogram truli
 	else
-		steps env defensivememop myprog falsli 
+		steps env defensivememop myprogram falsli 
   |Assign (reg, e) ->
 	let value = eval env e in
         let regname = get_register_name reg in
-        let env' = update regname value in
+        let env' = update regname value env in
 	 env'
 
  | Jump e -> 
 	let value = eval env e in
-	let env' = update "rip" value in 
+	let env' = update "rip" value env in 
 	(* FIXME: what about checks for jump?? *)
 	env'
 
- | Return -> let rsp = eval env (Register "rsp") in
-	     let rsp' = rsp - 1 in
-		update "rsp" rsp' 
+ | Return -> let rspvalue = eval env (Register "rsp") in
+	     let rspvalue' = (sub rspvalue 1uL) in
+		update "rsp" rspvalue' env
 
-and steps (env:cpuregstate) (defensivememop:memaccess) myprogram instrlist = List.fold_right (fun elem env' ->step env' defensivememop myprogram elem) instrlist env  
+and helperfunc  (defensivememop:memaccess) (myprogram:program) (elem:stmt) (env':cpuregstate): STL cpuregstate 
+					(requires (fun h -> true))
+					(ensures (fun h0 r h1 -> false)) =
+					step env' defensivememop myprogram elem 
+
+and steps (env:cpuregstate) (defensivememop:memaccess) myprogram instrlist = fold_right   (helperfunc defensivememop myprogram) instrlist env  
 
 (* Should the following function have a type that uses effects associated with effect ST ?  *)
-val ustar: (buffer dword)->address ->address->address->address->address->address->program->ST cpuregstate
-let ustar calltable base wbmapstart uheapstart ustackstart ucodestart entry myprogram = 
-  let memsize = 1000 in
-  let regsize = 1000 in
-  let buf = create  0uy memsize in 
-
+val ustar:(buffer dword)->(buffer dword)->address ->address->address->address->address->address->program->STL cpuregstate
+	(requires (fun h-> True))
+	(ensures (fun h0 r h1 -> True))
+let ustar buf calltable base wbmapstart uheapstart ustackstart ucodestart entry myprogram = 
   (* Modeling registers as list?? *)
-  let regslist = [MkReg "rsp" 0uy; MkReg "rbp" 0uy; MkReg "rip"  0uy; MkReg "rax" 0uy] in
+  let regslist = [MkReg "rsp" 0uL; MkReg "rbp" 0uL; MkReg "rip"  0uL; MkReg "rax" 0uL] in
   let mem = defensive buf calltable base wbmapstart ucodestart uheapstart ustackstart in
   let stmtlist = mem.decode myprogram entry in
   steps (Mkcpuregstate regslist) mem  myprogram stmtlist
